A new version of red-black trees (using the All-based definition of isBST). Some missing proofs here and there.

Data/EBTree.v
@@ -7,6 +7,37 @@ Inductive EBTree (M A : Type) : Type :=
 Arguments E {M A}.
 Arguments N {M A} _ _ _ _.
 
+(** * Function definitions *)
+
+Definition isEmpty {M A : Type} (t : EBTree M A) : bool :=
+match t with
+    | E => true
+    | _ => false
+end.
+
+Fixpoint height {M A : Type} (t : EBTree M A) : nat :=
+match t with
+    | E => 0
+    | N _ l _ r => 1 + max (height l) (height r)
+end.
+
+Fixpoint toList {M A : Type} (t : EBTree M A) : list A :=
+match t with
+    | E => []
+    | N _ l v r => toList l ++ v :: toList r
+end.
+
+Fixpoint countEBT {M A : Type} (p : A -> bool) (t : EBTree M A) : nat :=
+match t with
+    | E => 0
+    | N _ l v r =>
+        (if p v then 1 else 0) + countEBT p l + countEBT p r
+end.
+
+(** * Predicates and relations *)
+
+(** ** Elem *)
+
 Inductive Elem {M A : Type} (x : A) : EBTree M A -> Prop :=
     | Elem_root :
         forall (m : M) (l r : EBTree M A),
@@ -60,35 +91,103 @@ repeat match goal with
         specialize (H1 _ H2)
 end; auto.
 
-(* Inductive isBST {A : Ord} : EBTree M A -> Prop :=
+(** ** Ex *)
+
+Inductive Ex {M A : Type} (P : A -> Prop) : EBTree M A -> Type :=
+    | Ex_here :
+        forall (m : M) (v : A) (l r : EBTree M A),
+          P v -> Ex P (N m l v r)
+    | Ex_left :
+        forall (m : M) (v : A) (l r : EBTree M A),
+          Ex P l -> Ex P (N m l v r)
+    | Ex_right :
+        forall (m : M) (v : A) (l r : EBTree M A),
+          Ex P r -> Ex P (N m l v r).
+
+(** ** All *)
+
+Inductive All {M A : Type} (P : A -> Prop) : EBTree M A -> Prop :=
+    | All_E : All P E
+    | All_N :
+        forall (m : M) (l : EBTree M A) (v : A) (r : EBTree M A),
+          All P l -> P v -> All P r -> All P (N m l v r).
+
+Hint Constructors All : core.
+
+Ltac All :=
+repeat match goal with
+    | H : All _ E           |- _       => clear H
+    | H : All _ (N _ _ _ _) |- _       => inv H
+    |                       |- All _ E => constructor
+end.
+
+Ltac All' :=
+repeat match goal with
+    | H : All _ E           |- _       => clear H
+    | H : All _ (N _ _ _ _) |- _       => inv H
+    |                       |- All _ _ => constructor; auto
+end.
+
+(** ** isBST *)
+
+Require Import Ord.
+
+Inductive isBST {M : Type} {A : Ord} : EBTree M A -> Prop :=
     | isBST_E : isBST E
-    | isBST_T : forall (c : color) (v : A) (l r : EBTree M A),
-        (forall x : A, Elem x l -> x ≤ v) -> isBST l ->
-        (forall x : A, Elem x r -> v ≤ x) -> isBST r ->
-        isBST (T c l v r).
- *)
-Definition isEmpty {M A : Type} (t : EBTree M A) : bool :=
-match t with
-    | E => true
-    | _ => false
+    | isBST_N :
+        forall (m : M) (v : A) (l r : EBTree M A),
+          (forall x : A, Elem x l -> x ≤ v) -> isBST l ->
+          (forall x : A, Elem x r -> x >= v) -> isBST r ->
+            isBST (N m l v r).
+
+Hint Constructors isBST : core.
+
+Ltac isBST :=
+repeat match goal with
+    | H : isBST E           |- _       => clear H
+    | H : isBST (N _ _ _ _) |- _       => inv H
+    |                       |- isBST E => constructor
 end.
 
-Fixpoint height {M A : Type} (t : EBTree M A) : nat :=
-match t with
-    | E => 0
-    | N _ l _ r => 1 + max (height l) (height r)
+Ltac isBST' :=
+repeat match goal with
+    | H : isBST E           |- _       => clear H
+    | H : isBST (N _ _ _ _) |- _       => inv H
+    |                       |- isBST _ => constructor; intros; auto
 end.
 
-Function toList {M A : Type} (t : EBTree M A) : list A :=
-match t with
-    | E => []
-    | N _ l v r => toList l ++ v :: toList r
+(** ** isBST2 *)
+
+Inductive isBST2 {M : Type} {A : Ord} : EBTree M A -> Prop :=
+    | isBST2_E : isBST2 E
+    | isBST2_N : forall (m : M) (v : A) (l r : EBTree M A),
+        All (fun x : A => x ≤ v) l -> All (fun x : A => x >= v) r ->
+          isBST2 l -> isBST2 r -> isBST2 (N m l v r).
+
+Hint Constructors isBST2 : core.
+
+Ltac isBST2 :=
+repeat match goal with
+    | H : isBST2 E           |- _       => clear H
+    | H : isBST2 (N _ _ _ _) |- _       => inv H
+    |                       |- isBST2 E => constructor
+    | H : All _ E           |- _       => clear H
+    | H : All _ (N _ _ _ _) |- _       => inv H
 end.
 
-Fixpoint countEBT {M A : Type} (p : A -> bool) (t : EBTree M A) : nat :=
-match t with
-    | E => 0
-    | N _ l v r =>
-(*         (if p v then S else id) (countEBT p l + countEBT p r) *)
-        (if p v then 1 else 0) + countEBT p l + countEBT p r
+Ltac isBST2' :=
+repeat match goal with
+    | H : isBST2 E           |- _       => clear H
+    | H : isBST2 (N _ _ _ _) |- _       => inv H
+    |                       |- isBST2 _ => constructor; intros; auto
+    | H : All _ E           |- _       => clear H
+    | H : All _ (N _ _ _ _) |- _       => inv H
+    |                       |- All _ _ => constructor; auto
 end.
+
+Lemma All_Elem :
+  forall {M : Type} {A : Type} {P : A -> Prop} {t : EBTree M A},
+    All P t -> forall x : A, Elem x t -> P x.
+Proof.
+  induction 1; inv 1.
+Qed.
